LogicalRefinement/Stlc/InterpSubst.lean
@@ -281,6 +281,7 @@ theorem Term.term_subst_stlc_commute {Γ Δ σ a}
             rw [Subst.stlc_lift_true]
             rw [Subst.stlc_lift_false]
     case nz => cases H
+    case let_bin_delta => cases H
   }
 
 abbrev SubstCtx.interp {σ Γ Δ} (S: SubstCtx σ Γ Δ) (IΔ: IsCtx Δ)
